dsn/Lang/Prod/Basic.lean
@@ -8,240 +8,237 @@ namespace Lang
 
 --------------------------
 
-
-def ListPair.dom {α} {β} : List (α × β) → List α
-| .nil => .nil
-| (a, _) :: xs => a :: dom xs
+def Prod.dom (xs : List (α × β)) :=
+  List.map Prod.fst xs
 
 
-def remove {α} (id : String) : List (String × α) →  List (String × α)
-| .nil => .nil
-| (key, e) :: m =>
-  if key == id then
-    m
-  else
-    (key, e) :: (remove id m)
+def Prod.remove [BEq α] (target : α) (xs : List (α × β)) : List (α × β)
+:= List.filter (fun (key,_) => key != target) xs
 
-def remove_all {α} (m : List (String × α)) : (ids : List String) →  List (String × α)
-| .nil => m
-| id :: remainder => remove_all (remove id m) remainder
+def Prod.remove_all [BEq α] (xs : List (α × β)) : List α → List (α × β)
+| [] => xs
+| target :: targets => remove_all (Prod.remove target xs) targets
 
-def find {α} (id : String) : List (String × α) → Option α
-| .nil => none
-| (key, e) :: m =>
-  if key == id then
-    some e
-  else
-    find id m
+def Prod.find [BEq α] (target : α) (xs : List (α × β)) : Option β :=
+  Option.map Prod.snd (List.find? (fun (key,_) => key == target) xs)
+
+
+-- def find (target : String) : List (String × α) → Option α
+-- | .nil => none
+-- | (key, e) :: m =>
+--   if key == target then
+--     some e
+--   else
+--     find target m
 
 
 
-theorem ListPair.mem_concat_disj {β}
-  (x : String) (am0 am1 : List (String × β))
-:
-  x ∈ ListPair.dom (am1 ++ am0) →
-  x ∈ ListPair.dom am1 ∨ x ∈ ListPair.dom am0
-:= by induction am1 with
-  | nil =>
-    simp [dom]
-  | cons a am1' ih =>
-    simp [dom]
-    intro p
-    cases p with
-    | inl h =>
-      simp [*]
-    | inr h =>
-      have h := ih h
-      cases h with
-      | inl h' =>
-        simp [*]
-      | inr h' =>
-        simp [*]
+-- theorem ListPair.mem_concat_disj {β}
+--   (x : String) (am0 am1 : List (String × β))
+-- :
+--   x ∈ ListPair.dom (am1 ++ am0) →
+--   x ∈ ListPair.dom am1 ∨ x ∈ ListPair.dom am0
+-- := by induction am1 with
+--   | nil =>
+--     simp [dom]
+--   | cons a am1' ih =>
+--     simp [dom]
+--     intro p
+--     cases p with
+--     | inl h =>
+--       simp [*]
+--     | inr h =>
+--       have h := ih h
+--       cases h with
+--       | inl h' =>
+--         simp [*]
+--       | inr h' =>
+--         simp [*]
 
-theorem ListPair.mem_disj_concat_left {β}
-  (x : String) (am0 am1 : List (String × β))
-:
-  x ∈ ListPair.dom am1 →
-  x ∈ ListPair.dom (am1 ++ am0)
-:= by induction am1 with
-  | nil => simp [dom]
-  | cons a am1' ih =>
-    simp [dom]
-    intro p
-    cases p with
-    | inl h =>
-      simp [*]
-    | inr h =>
-      have h := ih h
-      simp [*]
+-- theorem ListPair.mem_disj_concat_left {β}
+--   (x : String) (am0 am1 : List (String × β))
+-- :
+--   x ∈ ListPair.dom am1 →
+--   x ∈ ListPair.dom (am1 ++ am0)
+-- := by induction am1 with
+--   | nil => simp [dom]
+--   | cons a am1' ih =>
+--     simp [dom]
+--     intro p
+--     cases p with
+--     | inl h =>
+--       simp [*]
+--     | inr h =>
+--       have h := ih h
+--       simp [*]
 
-theorem ListPair.mem_disj_concat_right {β}
-  (x : String) (am0 am1 : List (String × β))
-:
-  x ∈ ListPair.dom am0 →
-  x ∈ ListPair.dom (am1 ++ am0)
-:= by induction am1 with
-  | nil => simp
-  | cons a am1' ih =>
-    simp [dom]
-    intro p
-    have p := ih p
-    simp [*]
-
-
-theorem removeAll_refl {α} [BEq α] {xs ys : List α}:
-   List.removeAll xs ys ⊆ xs
-:= by sorry
-
-theorem containment_removeAll_concat_elim {α} [BEq α] {xs ys : List α}:
-   List.removeAll (xs ++ ys) ys ⊆ xs
-:= by sorry
-
-theorem containment_removeAll_union_elim {α} [BEq α] {xs ys : List α}:
-   List.removeAll (xs ∪ ys) ys ⊆ xs
-:= by sorry
+-- theorem ListPair.mem_disj_concat_right {β}
+--   (x : String) (am0 am1 : List (String × β))
+-- :
+--   x ∈ ListPair.dom am0 →
+--   x ∈ ListPair.dom (am1 ++ am0)
+-- := by induction am1 with
+--   | nil => simp
+--   | cons a am1' ih =>
+--     simp [dom]
+--     intro p
+--     have p := ih p
+--     simp [*]
 
 
-theorem removeAll_right_sub_cons_eq y {xs ys : List String} :
-  y ∈ ys → List.removeAll xs ys = List.removeAll xs (y :: ys)
-:= by sorry
+-- theorem removeAll_refl {α} [BEq α] {xs ys : List α}:
+--    List.removeAll xs ys ⊆ xs
+-- := by sorry
 
-theorem removeAll_left_sub_refl_disjoint {xs ys : List String} :
-  List.removeAll xs ys ∩ ys = []
-:= by sorry
+-- theorem containment_removeAll_concat_elim {α} [BEq α] {xs ys : List α}:
+--    List.removeAll (xs ++ ys) ys ⊆ xs
+-- := by sorry
 
-
-theorem removeAll_concat_eq {xs ys zs : List String} :
-  ys ⊆ zs →
-  List.removeAll xs zs = List.removeAll xs (ys ++ zs)
-:= by induction ys with
-  | nil =>
-    simp
-  | cons y ys' ih =>
-    intro ss
-    have p0 : y ∈ zs := by
-      apply ss
-      exact List.mem_cons_self
-    have p1 : ys' ⊆ zs := by
-      intro x m
-      apply ss
-      exact List.mem_cons_of_mem y m
-    rw [ih p1]
-    apply removeAll_right_sub_cons_eq
-    exact List.mem_append_right ys' p0
-
-theorem removeAll_concat_containment_left {xs ys zs : List String} :
-  List.removeAll xs (ys ++ zs) ⊆ List.removeAll xs ys
-:= by sorry
-
-theorem removeAll_concat_containment_right {xs ys zs : List String} :
-  List.removeAll xs (ys ++ zs) ⊆ List.removeAll xs zs
-:= by sorry
+-- theorem containment_removeAll_union_elim {α} [BEq α] {xs ys : List α}:
+--    List.removeAll (xs ∪ ys) ys ⊆ xs
+-- := by sorry
 
 
-theorem concat_right_containment {xs ys zs : List String} :
-  (xs ++ ys) ⊆ zs → ys ⊆ zs
-:= by
-  intro p0
-  intro a p1
-  apply p0
-  exact List.mem_append_right xs p1
+-- theorem removeAll_right_sub_cons_eq y {xs ys : List String} :
+--   y ∈ ys → List.removeAll xs ys = List.removeAll xs (y :: ys)
+-- := by sorry
+
+-- theorem removeAll_left_sub_refl_disjoint {xs ys : List String} :
+--   List.removeAll xs ys ∩ ys = []
+-- := by sorry
 
 
-theorem removeAll_decreasing_containment {xs ys zs : List String} :
-ys ⊆ zs → List.removeAll xs zs ⊆ List.removeAll xs ys
-:= by
-  intro ss
-  intro x dz
-  apply removeAll_concat_containment_left
-  rw [← removeAll_concat_eq] <;> assumption
+-- theorem removeAll_concat_eq {xs ys zs : List String} :
+--   ys ⊆ zs →
+--   List.removeAll xs zs = List.removeAll xs (ys ++ zs)
+-- := by induction ys with
+--   | nil =>
+--     simp
+--   | cons y ys' ih =>
+--     intro ss
+--     have p0 : y ∈ zs := by
+--       apply ss
+--       exact List.mem_cons_self
+--     have p1 : ys' ⊆ zs := by
+--       intro x m
+--       apply ss
+--       exact List.mem_cons_of_mem y m
+--     rw [ih p1]
+--     apply removeAll_right_sub_cons_eq
+--     exact List.mem_append_right ys' p0
+
+-- theorem removeAll_concat_containment_left {xs ys zs : List String} :
+--   List.removeAll xs (ys ++ zs) ⊆ List.removeAll xs ys
+-- := by sorry
+
+-- theorem removeAll_concat_containment_right {xs ys zs : List String} :
+--   List.removeAll xs (ys ++ zs) ⊆ List.removeAll xs zs
+-- := by sorry
 
 
-theorem removeAll_increasing_containment {xs : List String} :
-  ∀ ys zs, ys ⊆ zs → List.removeAll ys xs ⊆ List.removeAll zs xs
-:= by induction xs with
-  | nil =>
-    simp [List.removeAll]
-    exact fun ys zs a ↦ List.filter_subset (fun x ↦ true) a
-  | cons x xs ih =>
-    intro ys zs ss
-    simp [List.removeAll]
-    exact List.filter_subset (fun x_1 ↦ !decide (x_1 = x) && !decide (x_1 ∈ xs)) ss
+-- theorem concat_right_containment {xs ys zs : List String} :
+--   (xs ++ ys) ⊆ zs → ys ⊆ zs
+-- := by
+--   intro p0
+--   intro a p1
+--   apply p0
+--   exact List.mem_append_right xs p1
 
 
-theorem dom_concat_removeAll_containment {β} {am0 am1 : List (String × β)} {xs xs_im xs'} :
-  xs ⊆ xs_im → ListPair.dom am0 ⊆ List.removeAll xs_im xs →
-  xs_im ⊆ xs' → ListPair.dom am1 ⊆ List.removeAll xs' xs_im →
-  ListPair.dom (am1 ++ am0) ⊆ List.removeAll xs' xs
-:= by
-  intros ss0 dd0 ss1 dd1
-  induction am1 with
-  | nil =>
-    simp [*]
-    have ss1' : List.removeAll xs_im xs ⊆ List.removeAll xs' xs := by
-      apply removeAll_increasing_containment; simp [*]
-    intro x p
-    apply ss1'
-    apply dd0
-    simp [*]
-  |cons a am1' ih =>
-    let (x, v) := a
-    simp [ListPair.dom]
-    apply And.intro
-    {
-      apply removeAll_decreasing_containment ss0
-      apply dd1
-      simp [ListPair.dom]
-    }
-    {
-      apply ih
-      intro y1 p1
-      apply dd1
-      simp [ListPair.dom]
-      apply Or.inr
-      assumption
-    }
+-- theorem removeAll_decreasing_containment {xs ys zs : List String} :
+-- ys ⊆ zs → List.removeAll xs zs ⊆ List.removeAll xs ys
+-- := by
+--   intro ss
+--   intro x dz
+--   apply removeAll_concat_containment_left
+--   rw [← removeAll_concat_eq] <;> assumption
 
-theorem remove_all_empty α ids:
-  @remove_all α [] ids = []
-:= by induction ids with
-| nil =>
-  simp [remove_all]
-| cons id ids' ih =>
-  simp [remove_all, remove]
-  exact ih
 
-theorem remove_all_single_membership :
-  x ∈ ids →
-  remove_all [(x,c)] ids = []
-:= by induction ids with
-| nil =>
-  simp [remove_all]
-| cons id ids' ih =>
-  simp [remove_all]
-  intro h0
-  cases h0 with
-  | inl h1 =>
-    simp [*, remove]
-    simp [remove_all_empty]
-  | inr h1 =>
-    specialize ih h1
-    simp [remove]
-    by_cases h2 : x = id
-    { simp [h2,remove_all_empty] }
-    { simp [h2,ih] }
+-- theorem removeAll_increasing_containment {xs : List String} :
+--   ∀ ys zs, ys ⊆ zs → List.removeAll ys xs ⊆ List.removeAll zs xs
+-- := by induction xs with
+--   | nil =>
+--     simp [List.removeAll]
+--     exact fun ys zs a ↦ List.filter_subset (fun x ↦ true) a
+--   | cons x xs ih =>
+--     intro ys zs ss
+--     simp [List.removeAll]
+--     exact List.filter_subset (fun x_1 ↦ !decide (x_1 = x) && !decide (x_1 ∈ xs)) ss
 
-theorem remove_all_single_nomem :
-  x ∉ ids →
-  remove_all [(x,c)] ids = [(x,c)]
-:= by induction ids with
-| nil =>
-  simp [remove_all]
-| cons id ids ih =>
-  simp [remove_all,remove]
-  intro h0 h1
-  simp [h0]
-  apply ih h1
+
+-- theorem dom_concat_removeAll_containment {β} {am0 am1 : List (String × β)} {xs xs_im xs'} :
+--   xs ⊆ xs_im → ListPair.dom am0 ⊆ List.removeAll xs_im xs →
+--   xs_im ⊆ xs' → ListPair.dom am1 ⊆ List.removeAll xs' xs_im →
+--   ListPair.dom (am1 ++ am0) ⊆ List.removeAll xs' xs
+-- := by
+--   intros ss0 dd0 ss1 dd1
+--   induction am1 with
+--   | nil =>
+--     simp [*]
+--     have ss1' : List.removeAll xs_im xs ⊆ List.removeAll xs' xs := by
+--       apply removeAll_increasing_containment; simp [*]
+--     intro x p
+--     apply ss1'
+--     apply dd0
+--     simp [*]
+--   |cons a am1' ih =>
+--     let (x, v) := a
+--     simp [ListPair.dom]
+--     apply And.intro
+--     {
+--       apply removeAll_decreasing_containment ss0
+--       apply dd1
+--       simp [ListPair.dom]
+--     }
+--     {
+--       apply ih
+--       intro y1 p1
+--       apply dd1
+--       simp [ListPair.dom]
+--       apply Or.inr
+--       assumption
+--     }
+
+-- theorem remove_all_empty α ids:
+--   @remove_all α [] ids = []
+-- := by induction ids with
+-- | nil =>
+--   simp [remove_all]
+-- | cons id ids' ih =>
+--   simp [remove_all, remove]
+--   exact ih
+
+-- theorem remove_all_single_membership :
+--   x ∈ ids →
+--   remove_all [(x,c)] ids = []
+-- := by induction ids with
+-- | nil =>
+--   simp [remove_all]
+-- | cons id ids' ih =>
+--   simp [remove_all]
+--   intro h0
+--   cases h0 with
+--   | inl h1 =>
+--     simp [*, remove]
+--     simp [remove_all_empty]
+--   | inr h1 =>
+--     specialize ih h1
+--     simp [remove]
+--     by_cases h2 : x = id
+--     { simp [h2,remove_all_empty] }
+--     { simp [h2,ih] }
+
+-- theorem remove_all_single_nomem :
+--   x ∉ ids →
+--   remove_all [(x,c)] ids = [(x,c)]
+-- := by induction ids with
+-- | nil =>
+--   simp [remove_all]
+-- | cons id ids ih =>
+--   simp [remove_all,remove]
+--   intro h0 h1
+--   simp [h0]
+--   apply ih h1
 
 
 
