dsn/Lang/List/Basic.lean
@@ -4,119 +4,10 @@ set_option pp.fieldNotation false
 
 namespace Lang
 
-
---------------------------
-
-
-
-theorem List.cons_containment {α} [BEq α] {x : α} {xs ys : List α} :
-  x :: xs  ⊆ ys → x ∈ ys ∧ xs ⊆ ys
-:= by
-  intro p0
-  apply And.intro
-  {
-    apply p0
-    simp [*]
-  }
-  {
-    intro y p1
-    apply p0
-    simp [*]
-  }
-
--- #print List.inter
-
-#print decide
-
-example {α} [DecidableEq α] (x : α) (xs : List α) :
-  List.contains xs x =  decide (x ∈ xs)
-:= by exact List.contains_eq_mem x xs
-
-
-theorem List.not_mem_cons {α} [BEq α] {x x': α} {xs : List α} :
-  x ∉ (x' :: xs) →
-  x ≠ x' ∧ x ∉ xs
-:= by intro p ; exact List.ne_and_not_mem_of_not_mem_cons p
-
--- set_option pp.notation false in
-theorem List.nonmem_to_disjoint_right {α} [DecidableEq α] (x : α) (xs : List α) :
-  x ∉ xs → xs ∩ [x] = []
-:= by
-  intro h
-  induction xs with
-  | nil => exact rfl
-  | cons y ys ih =>
-    simp [Inter.inter, List.inter]
-
-    have ⟨l,r⟩ := List.ne_and_not_mem_of_not_mem_cons h
-    apply And.intro
-    { exact id (Ne.symm l) }
-    { intros x'' p ; exact (ne_of_mem_of_not_mem p r) }
-
-
-theorem List.disjoint_preservation_left {α} [BEq α] {xs ys zs : List α} :
-  xs ⊆ ys → ys ∩ zs = [] → xs ∩ zs = []
-:= by
-  simp [Inter.inter, List.inter]
-  intro p0
-  induction xs with
-  | nil =>
-    intro p1; intro a;
-    intro p2
-    cases p2
-  | cons x xs' ih =>
-    intro p1
-    have ⟨p2, p3⟩ := List.cons_containment p0
-    intro a
-    intro p4
-    cases p4 with
-    | head =>
-      exact p1 x p2
-    | tail _ p5 =>
-      apply ih p3 p1
-      exact p5
-
-theorem List.disjoint_preservation_right {α} [BEq α] {xs ys zs : List α} :
-  ys ⊆ zs → xs ∩ zs = [] → xs ∩ ys = []
-:= by
-  simp [Inter.inter, List.inter]
-  intro p0
-  induction xs with
-  | nil =>
-    intro p1; intro a;
-    intro p2
-    cases p2
-  | cons x xs' ih =>
-    intro p1
-    sorry
-
-theorem List.disjoint_concat_right {α} [BEq α] {xs ys zs : List α} :
-  xs ∩ (ys ++ zs) = [] → xs ∩ ys = [] ∧ xs ∩ zs = []
-:= by sorry
-
-
-theorem List.inter_empty_eq_empty {α} [BEq α] {ys : List α} :
-  ys ∩ [] = []
-:= by
-  cases ys with
-  | nil => exact rfl
-  | cons x xs =>
-    simp [Inter.inter, List.inter]
-
-
-theorem List.disjoint_swap {α} [BEq α] {xs ys : List α} :
-  xs ∩ ys = [] → ys ∩ xs = []
-:= by
-  intros
-  induction xs with
-  | nil => exact inter_empty_eq_empty
-  | cons => sorry
-
-#check List.any
 -- The English word "any" does not hold quantification meaning; it is simply a predication of a collection.
--- the quantification of "any" can be inferred to me either all or exists dependeing on context and inflection.
-def List.exi.{u} {α : Type u} (l : List α) (p : α → Bool) : Bool := List.any l p
-
+-- the quantification of "any" can be inferred to me either all or exists depending on context and inflection.
+def List.exi (xs : List α) (condition : α → Bool) : Bool :=
+  List.any xs condition
 
 def List.firstIndexOf {α} [BEq α] (target : α) (l : List α) : Option Nat :=
   let ns := List.indexesOf target l
@@ -130,12 +21,124 @@ def List.firstIndexOf {α} [BEq α] (target : α) (l : List α) : Option Nat :=
     .none
 
 
-example (id : String) (xs ys : List String):
-  id ∈ (xs ∪ ys) →
-  id ∈ xs ∨ id ∈ ys
-:= by
-  intro h0
-  exact Iff.mp List.mem_union_iff h0
+
+
+--------------------------
+
+
+
+-- theorem List.cons_containment {α} [BEq α] {x : α} {xs ys : List α} :
+--   x :: xs  ⊆ ys → x ∈ ys ∧ xs ⊆ ys
+-- := by
+--   intro p0
+--   apply And.intro
+--   {
+--     apply p0
+--     simp [*]
+--   }
+--   {
+--     intro y p1
+--     apply p0
+--     simp [*]
+--   }
+
+-- -- #print List.inter
+
+-- #print decide
+
+-- example {α} [DecidableEq α] (x : α) (xs : List α) :
+--   List.contains xs x =  decide (x ∈ xs)
+-- := by exact List.contains_eq_mem x xs
+
+
+-- theorem List.not_mem_cons {α} [BEq α] {x x': α} {xs : List α} :
+--   x ∉ (x' :: xs) →
+--   x ≠ x' ∧ x ∉ xs
+-- := by intro p ; exact List.ne_and_not_mem_of_not_mem_cons p
+
+-- -- set_option pp.notation false in
+-- theorem List.nonmem_to_disjoint_right {α} [DecidableEq α] (x : α) (xs : List α) :
+--   x ∉ xs → xs ∩ [x] = []
+-- := by
+--   intro h
+--   induction xs with
+--   | nil => exact rfl
+--   | cons y ys ih =>
+--     simp [Inter.inter, List.inter]
+
+--     have ⟨l,r⟩ := List.ne_and_not_mem_of_not_mem_cons h
+--     apply And.intro
+--     { exact id (Ne.symm l) }
+--     { intros x'' p ; exact (ne_of_mem_of_not_mem p r) }
+
+
+-- theorem List.disjoint_preservation_left {α} [BEq α] {xs ys zs : List α} :
+--   xs ⊆ ys → ys ∩ zs = [] → xs ∩ zs = []
+-- := by
+--   simp [Inter.inter, List.inter]
+--   intro p0
+--   induction xs with
+--   | nil =>
+--     intro p1; intro a;
+--     intro p2
+--     cases p2
+--   | cons x xs' ih =>
+--     intro p1
+--     have ⟨p2, p3⟩ := List.cons_containment p0
+--     intro a
+--     intro p4
+--     cases p4 with
+--     | head =>
+--       exact p1 x p2
+--     | tail _ p5 =>
+--       apply ih p3 p1
+--       exact p5
+
+-- theorem List.disjoint_preservation_right {α} [BEq α] {xs ys zs : List α} :
+--   ys ⊆ zs → xs ∩ zs = [] → xs ∩ ys = []
+-- := by
+--   simp [Inter.inter, List.inter]
+--   intro p0
+--   induction xs with
+--   | nil =>
+--     intro p1; intro a;
+--     intro p2
+--     cases p2
+--   | cons x xs' ih =>
+--     intro p1
+--     sorry
+
+-- theorem List.disjoint_concat_right {α} [BEq α] {xs ys zs : List α} :
+--   xs ∩ (ys ++ zs) = [] → xs ∩ ys = [] ∧ xs ∩ zs = []
+-- := by sorry
+
+
+-- theorem List.inter_empty_eq_empty {α} [BEq α] {ys : List α} :
+--   ys ∩ [] = []
+-- := by
+--   cases ys with
+--   | nil => exact rfl
+--   | cons x xs =>
+--     simp [Inter.inter, List.inter]
+
+
+-- theorem List.disjoint_swap {α} [BEq α] {xs ys : List α} :
+--   xs ∩ ys = [] → ys ∩ xs = []
+-- := by
+--   intros
+--   induction xs with
+--   | nil => exact inter_empty_eq_empty
+--   | cons => sorry
+
+
+
+-- example (id : String) (xs ys : List String):
+--   id ∈ (xs ∪ ys) →
+--   id ∈ xs ∨ id ∈ ys
+-- := by
+--   intro h0
+--   exact Iff.mp List.mem_union_iff h0
+
 
 
 theorem List.get_none_add_preservation {α} (m : List α) (i : Nat) (i' : Nat):
